update

Coq/Software Foundation/K_rel.v
@@ -4,6 +4,9 @@
   2. reflexive relation
   3. Transitive Relations
   4. Symmetric and Antisymmetric Relations
+  5. Equivalence Relations
+  6. Partial Orders and Preorders
+  7. Reflexive, Transitive Closure
 
 *)
 
@@ -115,6 +118,91 @@ Qed.
 
 
 (* Symmetric and Antisymmetric Relations *)
+
+Definition symmetric {X: Type} (R: X -> X -> Prop) :=
+  forall x y, R x y -> R y x.
+
+Definition antisymmetric {X: Type} (R: X -> X -> Prop) :=
+  forall x y, R x y -> R y x -> x = y.
+
+
+Theorem le_not_symm : antisymmetric le.
+Proof.
+  unfold antisymmetric.
+  intros.
+  Admitted.
+
+
+
+(* Equivalence Relations *)
+Definition equivlence {X:Type} (R: X -> X -> Prop) :=
+  reflexive_relation R /\ symmetric R /\ transitive R.
+
+
+
+
+(* Partial Orders and Preorders *)
+(*
+A relation is a partial order when it's reflexive, 
+anti-symmetric, and transitive. In the Coq standard 
+library it's called just "order" for short.
+*)
+Definition order {X: Type} (R: relation X) :=
+  reflexive_relation R /\ transitive R /\ antisymmetric R.
+
+(* A preorder is almost like a partial order, 
+   but doesn't have to be antisymmetric.
+ *)
+Definition preorder {X:Type} (R: relation X) :=
+  reflexive_relation R /\ transitive R.
+
+Theorem le_order : order le.
+Proof.
+  unfold order.
+  split.
+    -apply le_reflexive.
+    -split.
+      +apply le_trans.
+      +apply le_not_symm.
+Qed.
+
+
+
+
+(* Reflexive, Transitive Closure *)
+(*
+The reflexive, transitive closure of a relation R is the smallest
+relation that contains R and that is both reflexive and transitive
+*)
+Inductive clos_refl_trans {X: Type} (R: relation X) : relation X :=
+| rt_step : forall x y, R x y -> clos_refl_trans R x y
+| rt_refl : forall x, clos_refl_trans R x x
+| rt_trans : forall x y z, clos_refl_trans R x y -> 
+                           clos_refl_trans R y z ->
+                           clos_refl_trans R x z.
+
+(*
+BTW:the reflexive and transitive closure of the next_nat 
+relation is the le relation.
+*)
+
+(*
+this definition is nature but not very convenient for 
+doing proofs, since the "nondeterminism" of the rt_trans 
+rule can sometimes lead to tricky inductions. Here is 
+a more useful definition:
+*)
+
+Inductive clos_refl_trans_1n {A: Type} (R: relation A) (x: A) : A -> Prop :=
+| rt1n_refl : clos_refl_trans_1n R x x
+| rt1n_trans (y z: A) : R x y -> clos_refl_trans_1n R y z -> 
+                                 clos_refl_trans_1n R x z.
+
+
+
+
+
+
 
 
 
