Coq/Software Foundation/M_stack_compiler.v
@@ -1,0 +1,171 @@
+
+Require Import H_maps.
+Require Import Coq.Lists.List.
+Require Import Coq.Arith.Arith.
+Require Import Coq.omega.Omega.
+Require Import PeanoNat.
+Import ListNotations.
+
+Definition state := total_map nat.  (* define state type *)
+Definition empty_state := t_empty 0.
+
+
+Definition W : id := Id "W".
+Definition X : id := Id "X".
+Definition Y : id := Id "Y".
+Definition Z : id := Id "Z".
+
+
+(* AST *)
+Inductive aexp : Type :=
+| ANum : nat -> aexp
+| AId  : id -> aexp
+| APlus   : aexp -> aexp -> aexp
+| AMult   : aexp -> aexp -> aexp
+| AMinus  : aexp -> aexp -> aexp.
+
+
+
+(* Instruction *)
+Inductive sinstr : Type :=
+| SPush : nat -> sinstr
+| SLoad : id -> sinstr
+| SPlus : sinstr
+| SMinus : sinstr
+| SMult : sinstr.
+
+
+
+(* compile *)
+Fixpoint s_compile (e : aexp) : list sinstr :=
+match e with
+| ANum n => [SPush n]
+| AId i => [SLoad i]
+| APlus a1 a2 => (s_compile a1) ++ (s_compile a2) ++ [SPlus]
+| AMult a1 a2 => (s_compile a1) ++ (s_compile a2) ++ [SMult]
+| AMinus a1 a2 => (s_compile a1) ++ (s_compile a2) ++ [SMinus]
+end.
+
+(* test *)
+Example s_compile1 :
+    s_compile (AMinus (AId X) (AMult (ANum 2) (AId Y)))
+  = [SLoad X; SPush 2; SLoad Y; SMult; SMinus].
+Proof.
+  simpl. auto.
+Qed.
+
+
+
+
+
+(* eval instruction *)
+Fixpoint s_execute (st : state) (stack : list nat)
+                   (prog : list sinstr) : list nat :=
+match prog with
+| [] => stack
+| inst :: ll => let sk' := match inst with
+                           | SPush n => n::stack
+                           | SLoad i => (st i)::stack
+                           | SPlus => match stack with
+                                      | x1::x2::xl => (x1 + x2)::xl
+                                      | _ => []
+                                      end
+                           | SMinus => match stack with
+                                       | x1::x2::xl => (x2 - x1)::xl
+                                       | _ => []
+                                       end
+                           | SMult => match stack with
+                                      | x1::x2::xl => (x1 * x2)::xl
+                                      | _ => []
+                                      end
+                           end
+                in (s_execute st sk' ll)
+end.
+
+(*test*)
+Example s_execute1 :
+     s_execute empty_state []
+       [SPush 5; SPush 3; SPush 1; SMinus]
+   = [2; 5].
+Proof.
+  simpl. auto.
+Qed.
+
+Example s_execute2 :
+     s_execute (t_update empty_state X 3) [3;4]
+       [SPush 4; SLoad X; SMult; SPlus]
+   = [15; 4].
+Proof.
+  simpl. auto.
+Qed.
+
+
+
+
+
+
+
+
+
+
+(* proof the correctness of the compiler *)
+Fixpoint aeval (st : state) (a : aexp) : nat := 
+    match a with
+    | ANum n => n
+    | AId id => st id
+    | APlus n m => (aeval st n) + (aeval st m)
+    | AMult n m => (aeval st n) * (aeval st m)
+    | AMinus n m => (aeval st n) - (aeval st m)
+    end.
+
+Lemma s_execute_app: forall st is1 is2 l,
+  s_execute st l (is1 ++ is2) = s_execute st (s_execute st l is1) is2.
+Proof.
+  intros st is1 is2.
+  induction is1 as [| i is1'].
+  -reflexivity.
+  -intros l. induction i;
+      simpl; apply IHis1'. 
+Qed.
+
+Theorem s_compile_correct_general : forall (st : state) (e : aexp) sk,
+  s_execute st sk (s_compile e) = [ aeval st e ] ++ sk.
+Proof.
+  intros.
+  generalize dependent sk.
+  induction e;
+  try(intros; simpl; auto);
+  try(repeat rewrite s_execute_app);
+  try(rewrite IHe1; rewrite IHe2; simpl);
+  try rewrite plus_comm; try rewrite mult_comm; auto.
+Qed.
+
+
+
+Theorem s_compile_correct : forall (st : state) (e : aexp),
+  s_execute st [] (s_compile e) = [ aeval st e ].
+Proof.
+  intros.
+  apply s_compile_correct_general.
+Qed.
+
+
+
+
+
+
+
+
+
+
+
+
+
+
+
+
+
+
+
+
+
